add nested array and record, re-do checks proof, simplify formalization,and so on

spark2014_semantics/spark2014_core_subset/checks_generator.v
@@ -1,4 +1,5 @@
 Require Export language_flagged.
+Require Export language_util.
 Require Export symboltable.
 
 (* ***************************************************************
@@ -39,67 +40,68 @@ Require Export symboltable.
                (the division check can also be removed, as (X + 1) > 0 )
 *)
 
-Inductive compile2_flagged_exp: symboltable -> check_flags -> expression -> expression_x -> Prop :=
-    | C2_Flagged_Literal: forall st checkflags ast_num l,
-        compile2_flagged_exp st checkflags 
-                             (E_Literal ast_num l) 
-                             (E_Literal_X ast_num l checkflags)
-    | C2_Flagged_Name: forall st checkflags n n_flagged ast_num,
-        compile2_flagged_name st checkflags n n_flagged -> (* checkflags for name expression is enforced on name n *)
-        compile2_flagged_exp st checkflags 
-                             (E_Name ast_num n) 
-                             (E_Name_X ast_num n_flagged nil)
-    | C2_Flagged_Binary_Operation_O: forall op st e1 e1_flagged e2 e2_flagged checkflags ast_num,
+Inductive compile2_flagged_exp: symboltable -> expression -> expression_x -> Prop :=
+    | C2_Flagged_Literal_Bool: forall st ast_num b,
+        compile2_flagged_exp st (E_Literal ast_num (Boolean_Literal b)) 
+                                (E_Literal_X ast_num (Boolean_Literal b) nil nil)
+    | C2_Flagged_Literal_Int_T: forall st v ast_num,
+        (Zge_bool v min_signed) && (Zle_bool v max_signed) = true -> (*simple optimization: if v is in the range of Integer, then no overflow check*)
+        compile2_flagged_exp st (E_Literal ast_num (Integer_Literal v)) 
+                                (E_Literal_X ast_num (Integer_Literal v) nil nil)
+    | C2_Flagged_Literal_Int_F: forall st v ast_num,
+        (Zge_bool v min_signed) && (Zle_bool v max_signed) = false ->
+        compile2_flagged_exp st (E_Literal ast_num (Integer_Literal v)) 
+                                (E_Literal_X ast_num (Integer_Literal v) (Do_Overflow_Check :: nil) nil)
+    | C2_Flagged_Name: forall st n n_flagged ast_num,
+        compile2_flagged_name st n n_flagged ->
+        compile2_flagged_exp st (E_Name ast_num n) 
+                                (E_Name_X ast_num n_flagged)
+    | C2_Flagged_Binary_Operation_O: forall st op e1 e1_flagged e2 e2_flagged ast_num,
         op = Plus \/ op = Minus \/ op = Multiply ->
-        compile2_flagged_exp st nil e1 e1_flagged ->
-        compile2_flagged_exp st nil e2 e2_flagged ->
-        compile2_flagged_exp st checkflags
-                             (E_Binary_Operation ast_num op e1 e2)
-                             (E_Binary_Operation_X ast_num op e1_flagged e2_flagged (Do_Overflow_Check :: checkflags))
-    | C2_Flagged_Binary_Operation_OD: forall op st e1 e1_flagged e2 e2_flagged checkflags ast_num,
+        compile2_flagged_exp st e1 e1_flagged ->
+        compile2_flagged_exp st e2 e2_flagged ->
+        compile2_flagged_exp st (E_Binary_Operation ast_num op e1 e2)
+                                (E_Binary_Operation_X ast_num op e1_flagged e2_flagged (Do_Overflow_Check :: nil) nil)
+    | C2_Flagged_Binary_Operation_OD: forall st op e1 e1_flagged e2 e2_flagged ast_num,
         op = Divide ->
-        compile2_flagged_exp st nil e1 e1_flagged ->
-        compile2_flagged_exp st nil e2 e2_flagged ->
-        compile2_flagged_exp st checkflags
-                             (E_Binary_Operation ast_num op e1 e2)
-                             (E_Binary_Operation_X ast_num op e1_flagged e2_flagged (Do_Division_Check :: Do_Overflow_Check :: checkflags))
-    | C2_Flagged_Binary_Operation_Others: forall op st e1 e1_flagged e2 e2_flagged checkflags ast_num,
+        compile2_flagged_exp st e1 e1_flagged ->
+        compile2_flagged_exp st e2 e2_flagged ->
+        compile2_flagged_exp st (E_Binary_Operation ast_num op e1 e2)
+                                (E_Binary_Operation_X ast_num op e1_flagged e2_flagged (Do_Division_Check :: Do_Overflow_Check :: nil) nil)
+    | C2_Flagged_Binary_Operation_Others: forall st op e1 e1_flagged e2 e2_flagged ast_num,
         op <> Plus ->
         op <> Minus ->
         op <> Multiply ->
         op <> Divide ->
-        compile2_flagged_exp st nil e1 e1_flagged ->
-        compile2_flagged_exp st nil e2 e2_flagged ->
-        compile2_flagged_exp st checkflags
-                             (E_Binary_Operation ast_num op e1 e2)
-                             (E_Binary_Operation_X ast_num op e1_flagged e2_flagged checkflags)
-    | C2_Flagged_Unary_Operation_O: forall op st e e_flagged checkflags ast_num,
+        compile2_flagged_exp st e1 e1_flagged ->
+        compile2_flagged_exp st e2 e2_flagged ->
+        compile2_flagged_exp st (E_Binary_Operation ast_num op e1 e2)
+                                (E_Binary_Operation_X ast_num op e1_flagged e2_flagged nil nil)
+    | C2_Flagged_Unary_Operation_O: forall st op e e_flagged ast_num,
         op = Unary_Minus ->
-        compile2_flagged_exp st nil e e_flagged ->
-        compile2_flagged_exp st checkflags
-                             (E_Unary_Operation ast_num op e) 
-                             (E_Unary_Operation_X ast_num op e_flagged (Do_Overflow_Check :: checkflags))
-    | C2_Flagged_Unary_Operation_Others: forall op st e e_flagged checkflags ast_num,
+        compile2_flagged_exp st e e_flagged ->
+        compile2_flagged_exp st (E_Unary_Operation ast_num op e) 
+                                (E_Unary_Operation_X ast_num op e_flagged (Do_Overflow_Check :: nil) nil)
+    | C2_Flagged_Unary_Operation_Others: forall st op e e_flagged ast_num,
         op <> Unary_Minus ->
-        compile2_flagged_exp st nil e e_flagged ->
-        compile2_flagged_exp st checkflags
-                             (E_Unary_Operation ast_num op e) 
-                             (E_Unary_Operation_X ast_num op e_flagged checkflags)
+        compile2_flagged_exp st e e_flagged ->
+        compile2_flagged_exp st (E_Unary_Operation ast_num op e) 
+                                (E_Unary_Operation_X ast_num op e_flagged nil nil)
 
-with compile2_flagged_name: symboltable -> check_flags -> name -> name_x -> Prop :=
-    | C2_Flagged_Identifier: forall st checkflags ast_num x,
-        compile2_flagged_name st checkflags 
-                              (E_Identifier ast_num x) 
-                              (E_Identifier_X ast_num x checkflags) 
-    | C2_Flagged_Indexed_Component: forall st e e_flagged checkflags ast_num x_ast_num x,
-        compile2_flagged_exp st (Do_Range_Check :: nil) e e_flagged ->
-        compile2_flagged_name st checkflags
-                              (E_Indexed_Component ast_num x_ast_num x e) 
-                              (E_Indexed_Component_X ast_num x_ast_num x e_flagged checkflags) 
-    | C2_Flagged_Selected_Component: forall st checkflags ast_num x_ast_num x f,
-        compile2_flagged_name st checkflags 
-                              (E_Selected_Component ast_num x_ast_num x f) 
-                              (E_Selected_Component_X ast_num x_ast_num x f checkflags).
+with compile2_flagged_name: symboltable -> name -> name_x -> Prop :=
+    | C2_Flagged_Identifier: forall st ast_num x,
+        compile2_flagged_name st (E_Identifier ast_num x) (* the value of x should be already checked before it's stored in memory, so no check is needed when it's read *)
+                                 (E_Identifier_X ast_num x nil) 
+    | C2_Flagged_Indexed_Component: forall st e e_flagged x x_flagged ast_num,
+        compile2_flagged_exp st e e_flagged ->
+        compile2_flagged_name st x x_flagged -> (* x itself can be an indexed/selected component *)
+        compile2_flagged_name st (E_Indexed_Component ast_num x e) 
+                                 (E_Indexed_Component_X ast_num x_flagged (update_exterior_checks_exp e_flagged (Do_Range_Check :: nil)) nil) 
+    | C2_Flagged_Selected_Component: forall st x x_flagged ast_num f,
+        compile2_flagged_name st x x_flagged ->
+        compile2_flagged_name st (E_Selected_Component ast_num x f) 
+                                 (E_Selected_Component_X ast_num x_flagged f nil).
+
 
 (**
    for a procedure call, during its copy in, Do_Range_Check should be performed 
@@ -122,61 +124,65 @@ Inductive compile2_flagged_args: symboltable -> list parameter_specification -> 
     | C2_Flagged_Args_In: forall st param arg arg_flagged lparam larg larg_flagged,
         param.(parameter_mode) = In ->
         is_range_constrainted_type (param.(parameter_subtype_mark)) = false ->
-        compile2_flagged_exp st nil arg arg_flagged ->
+        compile2_flagged_exp  st arg arg_flagged ->
         compile2_flagged_args st lparam larg larg_flagged -> 
         compile2_flagged_args st (param :: lparam) (arg :: larg) (arg_flagged :: larg_flagged)
-    | C2_Flagged_Args_In_Range: forall st param arg arg_flagged lparam larg larg_flagged,
+    | C2_Flagged_Args_In_RangeCheck: forall st param arg arg_flagged lparam larg larg_flagged,
         param.(parameter_mode) = In ->
         is_range_constrainted_type (param.(parameter_subtype_mark)) = true ->
-        compile2_flagged_exp st (Do_Range_Check :: nil) arg arg_flagged ->
+        compile2_flagged_exp  st arg arg_flagged ->
         compile2_flagged_args st lparam larg larg_flagged -> 
-        compile2_flagged_args st (param :: lparam) (arg :: larg) (arg_flagged :: larg_flagged)
-    | C2_Flagged_Args_Out: forall st param ast_num t x_ast_num x_flagged lparam larg larg_flagged x,
+        compile2_flagged_args st (param :: lparam) (arg :: larg) ((update_exterior_checks_exp arg_flagged (Do_Range_Check :: nil)) :: larg_flagged)
+    | C2_Flagged_Args_Out: forall st param ast_num t n_flagged lparam larg larg_flagged n,
         param.(parameter_mode) = Out ->
         fetch_exp_type ast_num st = Some t ->
         is_range_constrainted_type t = false ->
-        compile2_flagged_exp st nil (E_Name ast_num (E_Identifier x_ast_num x)) x_flagged ->
+        compile2_flagged_name st n n_flagged ->
         compile2_flagged_args st lparam larg larg_flagged -> 
-        compile2_flagged_args st (param :: lparam) ((E_Name ast_num (E_Identifier x_ast_num x)) :: larg) (x_flagged :: larg_flagged)
-    | C2_Flagged_Args_Out_Range: forall st param ast_num t x_ast_num x_flagged lparam larg larg_flagged x,
+        compile2_flagged_args st (param :: lparam) ((E_Name ast_num n) :: larg) ((E_Name_X ast_num n_flagged) :: larg_flagged)
+    | C2_Flagged_Args_Out_RangeCheck: forall st param ast_num t n_flagged lparam larg larg_flagged n,
         param.(parameter_mode) = Out ->
         fetch_exp_type ast_num st = Some t ->
         is_range_constrainted_type t = true ->
-        compile2_flagged_exp st (Do_Range_Check_On_CopyOut :: nil) (E_Name ast_num (E_Identifier x_ast_num x)) x_flagged ->
+        compile2_flagged_name st n n_flagged ->
         compile2_flagged_args st lparam larg larg_flagged -> 
-        compile2_flagged_args st (param :: lparam) ((E_Name ast_num (E_Identifier x_ast_num x)) :: larg) (x_flagged :: larg_flagged)
-    | C2_Flagged_Args_InOut: forall st param ast_num t x_ast_num x_flagged lparam larg larg_flagged x,
+        compile2_flagged_args st (param :: lparam) ((E_Name ast_num n) :: larg) 
+                                                   ((E_Name_X ast_num (update_exterior_checks_name n_flagged (Do_Range_Check_On_CopyOut :: nil))) :: larg_flagged)
+    | C2_Flagged_Args_InOut: forall st param ast_num t n_flagged lparam larg larg_flagged n,
         param.(parameter_mode) = In_Out ->
         is_range_constrainted_type (param.(parameter_subtype_mark)) = false ->
         fetch_exp_type ast_num st = Some t ->
         is_range_constrainted_type t = false ->
-        compile2_flagged_exp st nil (E_Name ast_num (E_Identifier x_ast_num x)) x_flagged ->
+        compile2_flagged_name st n n_flagged ->
         compile2_flagged_args st lparam larg larg_flagged -> 
-        compile2_flagged_args st (param :: lparam) ((E_Name ast_num (E_Identifier x_ast_num x)) :: larg) (x_flagged :: larg_flagged)
-    | C2_Flagged_Args_InOut_In_Range: forall st param ast_num t x_ast_num x_flagged lparam larg larg_flagged x,
+        compile2_flagged_args st (param :: lparam) ((E_Name ast_num n) :: larg) ((E_Name_X ast_num n_flagged) :: larg_flagged)
+    | C2_Flagged_Args_InOut_In_RangeCheck: forall st param ast_num t n_flagged lparam larg larg_flagged n,
         param.(parameter_mode) = In_Out ->
         is_range_constrainted_type (param.(parameter_subtype_mark)) = true ->
         fetch_exp_type ast_num st = Some t ->
         is_range_constrainted_type t = false ->
-        compile2_flagged_exp st (Do_Range_Check :: nil) (E_Name ast_num (E_Identifier x_ast_num x)) x_flagged ->
+        compile2_flagged_name st n n_flagged ->
         compile2_flagged_args st lparam larg larg_flagged -> 
-        compile2_flagged_args st (param :: lparam) ((E_Name ast_num (E_Identifier x_ast_num x)) :: larg) (x_flagged :: larg_flagged)
-    | C2_Flagged_Args_InOut_Out_Range: forall st param ast_num t x_ast_num x_flagged lparam larg larg_flagged x,
+        compile2_flagged_args st (param :: lparam) ((E_Name ast_num n) :: larg) 
+                                                   ((E_Name_X ast_num (update_exterior_checks_name n_flagged (Do_Range_Check :: nil))) :: larg_flagged)
+    | C2_Flagged_Args_InOut_Out_RangeCheck: forall st param ast_num t n_flagged lparam larg larg_flagged n,
         param.(parameter_mode) = In_Out ->
         is_range_constrainted_type (param.(parameter_subtype_mark)) = false ->
         fetch_exp_type ast_num st = Some t ->
         is_range_constrainted_type t = true ->
-        compile2_flagged_exp st (Do_Range_Check_On_CopyOut :: nil) (E_Name ast_num (E_Identifier x_ast_num x)) x_flagged ->
+        compile2_flagged_name st n n_flagged ->
         compile2_flagged_args st lparam larg larg_flagged -> 
-        compile2_flagged_args st (param :: lparam) ((E_Name ast_num (E_Identifier x_ast_num x)) :: larg) (x_flagged :: larg_flagged)
-    | C2_Flagged_Args_InOut_Range: forall st param ast_num t x_ast_num x_flagged lparam larg larg_flagged x,
+        compile2_flagged_args st (param :: lparam) ((E_Name ast_num n) :: larg) 
+                                                   ((E_Name_X ast_num (update_exterior_checks_name n_flagged (Do_Range_Check_On_CopyOut :: nil))) :: larg_flagged)
+    | C2_Flagged_Args_InOut_RangeCheck: forall st param ast_num t n_flagged lparam larg larg_flagged n,
         param.(parameter_mode) = In_Out ->
         is_range_constrainted_type (param.(parameter_subtype_mark)) = true ->
         fetch_exp_type ast_num st = Some t ->
         is_range_constrainted_type t = true ->
-        compile2_flagged_exp st (Do_Range_Check :: Do_Range_Check_On_CopyOut :: nil) (E_Name ast_num (E_Identifier x_ast_num x)) x_flagged ->
+        compile2_flagged_name st n n_flagged ->
         compile2_flagged_args st lparam larg larg_flagged -> 
-        compile2_flagged_args st (param :: lparam) ((E_Name ast_num (E_Identifier x_ast_num x)) :: larg) (x_flagged :: larg_flagged).
+        compile2_flagged_args st (param :: lparam) ((E_Name ast_num n) :: larg) 
+                                                   ((E_Name_X ast_num (update_exterior_checks_name n_flagged (Do_Range_Check :: Do_Range_Check_On_CopyOut :: nil))) :: larg_flagged).
 
 
 (**
@@ -190,28 +196,28 @@ Inductive compile2_flagged_stmt: symboltable -> statement -> statement_x -> Prop
     | C2_Flagged_Assignment: forall x st t x_flagged e e_flagged ast_num,
         fetch_exp_type (name_astnum x) st = Some t ->
         is_range_constrainted_type t = false ->        
-        compile2_flagged_name st nil x x_flagged ->
-        compile2_flagged_exp  st nil e e_flagged ->
+        compile2_flagged_name st x x_flagged ->
+        compile2_flagged_exp  st e e_flagged ->
         compile2_flagged_stmt st
                               (S_Assignment   ast_num x e) 
                               (S_Assignment_X ast_num x_flagged e_flagged)
-    | C2_Flagged_Assignment_R: forall x st t x_flagged e e_flagged ast_num,
+    | C2_Flagged_Assignment_RangeCheck: forall x st t x_flagged e e_flagged ast_num,
         fetch_exp_type (name_astnum x) st = Some t ->
         is_range_constrainted_type t = true ->
-        compile2_flagged_name st nil x x_flagged ->
-        compile2_flagged_exp  st (Do_Range_Check :: nil) e e_flagged ->
+        compile2_flagged_name st x x_flagged ->
+        compile2_flagged_exp  st e e_flagged ->
         compile2_flagged_stmt st
                               (S_Assignment   ast_num x e)
-                              (S_Assignment_X ast_num x_flagged e_flagged)
-    | C2_Flagged_If: forall e e_flagged c1 c1_flagged c2 c2_flagged st ast_num,
-        compile2_flagged_exp  st nil e e_flagged ->
+                              (S_Assignment_X ast_num x_flagged (update_exterior_checks_exp e_flagged (Do_Range_Check :: nil)))
+    | C2_Flagged_If: forall e e_flagged st c1 c1_flagged c2 c2_flagged ast_num,
+        compile2_flagged_exp  st e e_flagged ->
         compile2_flagged_stmt st c1 c1_flagged ->
         compile2_flagged_stmt st c2 c2_flagged ->
         compile2_flagged_stmt st
                               (S_If   ast_num e c1 c2) 
                               (S_If_X ast_num e_flagged c1_flagged c2_flagged)
-    | C2_Flagged_While: forall e e_flagged c c_flagged st ast_num,
-        compile2_flagged_exp  st nil e e_flagged ->
+    | C2_Flagged_While: forall e e_flagged st c c_flagged ast_num,
+        compile2_flagged_exp  st e e_flagged ->
         compile2_flagged_stmt st c c_flagged ->
         compile2_flagged_stmt st 
                               (S_While_Loop   ast_num e c) 
@@ -242,10 +248,10 @@ Inductive compile2_flagged_type_declaration: type_declaration -> type_declaratio
         compile2_flagged_type_declaration (Integer_Type_Declaration   ast_num tn (Range l u))
                                           (Integer_Type_Declaration_X ast_num tn (Range_X l u))
     | C2_Flagged_Array_Type_Decl: forall ast_num tn tm t,
-        compile2_flagged_type_declaration (Array_Type_Declaration   ast_num tn tm t)
+        compile2_flagged_type_declaration (Array_Type_Declaration   ast_num tn tm t) (* tn: array type name, tm: index type mark, t: component type *)
                                           (Array_Type_Declaration_X ast_num tn tm t)
     | C2_Flagged_Record_Type_Decl: forall ast_num tn fs,
-        compile2_flagged_type_declaration (Record_Type_Declaration   ast_num tn fs) 
+        compile2_flagged_type_declaration (Record_Type_Declaration   ast_num tn fs)  (* tn: record type name, fs: list of field types *)
                                           (Record_Type_Declaration_X ast_num tn fs).
 
 (** insert run-time check flags on the initialization expression 
@@ -258,16 +264,16 @@ Inductive compile2_flagged_object_declaration: symboltable -> object_declaration
                                             (mkobject_declaration_x ast_num x t None) 
     | C2_Flagged_Object_Declaration: forall st t e e_flagged ast_num x,
         is_range_constrainted_type t = false ->
-        compile2_flagged_exp st nil e e_flagged ->
+        compile2_flagged_exp st e e_flagged ->
         compile2_flagged_object_declaration st 
-                                            (mkobject_declaration   ast_num x t (Some e)) 
+                                            (mkobject_declaration   ast_num x t (Some e)) (* declare a variable x of type t with initialization e *)
                                             (mkobject_declaration_x ast_num x t (Some e_flagged))
-    | C2_Flagged_Object_Declaration_R: forall st t e e_flagged ast_num x,
+    | C2_Flagged_Object_Declaration_RangeCheck: forall st t e e_flagged ast_num x,
         is_range_constrainted_type t = true ->
-        compile2_flagged_exp st (Do_Range_Check :: nil) e e_flagged ->
+        compile2_flagged_exp st e e_flagged ->
         compile2_flagged_object_declaration st 
                                             (mkobject_declaration   ast_num x t (Some e)) 
-                                            (mkobject_declaration_x ast_num x t (Some e_flagged)).
+                                            (mkobject_declaration_x ast_num x t (Some (update_exterior_checks_exp e_flagged (Do_Range_Check :: nil)))).
 
 Inductive compile2_flagged_object_declarations: symboltable -> list object_declaration -> list object_declaration_x -> Prop :=
     | C2_Flagged_Object_Declarations_Null: forall st,
@@ -280,7 +286,7 @@ Inductive compile2_flagged_object_declarations: symboltable -> list object_decla
 
 Inductive compile2_flagged_parameter_specification: parameter_specification -> parameter_specification_x -> Prop :=
     | C2_Flagged_Parameter_Spec: forall ast_num x t m,
-        compile2_flagged_parameter_specification (mkparameter_specification   ast_num x t m)
+        compile2_flagged_parameter_specification (mkparameter_specification   ast_num x t m) (* a parameter x of type t of in/out mode m *)
                                                  (mkparameter_specification_x ast_num x t m).
 
 Inductive compile2_flagged_parameter_specifications: list parameter_specification -> list parameter_specification_x -> Prop :=
@@ -334,126 +340,98 @@ with compile2_flagged_procedure_body: symboltable -> procedure_body -> procedure
 
 (** * Functions for Inserting Run-Time Checks *)
 
-Function compile2_flagged_exp_f (st: symboltable) (checkflags: check_flags) (e: expression): expression_x :=
+Function compile2_flagged_exp_f (st: symboltable) (e: expression): expression_x :=
   match e with
-  | E_Literal ast_num l => 
-        E_Literal_X ast_num l checkflags
+  | E_Literal ast_num (Boolean_Literal b) => 
+      E_Literal_X ast_num (Boolean_Literal b) nil nil
+  | E_Literal ast_num (Integer_Literal v) =>
+      match (Zge_bool v min_signed) && (Zle_bool v max_signed) with
+      | true  => E_Literal_X ast_num (Integer_Literal v) nil nil (* optimization *)
+      | false => E_Literal_X ast_num (Integer_Literal v) (Do_Overflow_Check :: nil) nil
+      end
   | E_Name ast_num n => 
-      let n_flagged := compile2_flagged_name_f st checkflags n in
-        E_Name_X ast_num n_flagged nil
+      let n_flagged := compile2_flagged_name_f st n in
+        E_Name_X ast_num n_flagged
   | E_Binary_Operation ast_num op e1 e2 =>
-      let e1_flagged := compile2_flagged_exp_f st nil e1 in
-      let e2_flagged := compile2_flagged_exp_f st nil e2 in
+      let e1_flagged := compile2_flagged_exp_f st e1 in
+      let e2_flagged := compile2_flagged_exp_f st e2 in
         match op with
-        | Plus     => E_Binary_Operation_X ast_num op e1_flagged e2_flagged (Do_Overflow_Check :: checkflags)
-        | Minus    => E_Binary_Operation_X ast_num op e1_flagged e2_flagged (Do_Overflow_Check :: checkflags)
-        | Multiply => E_Binary_Operation_X ast_num op e1_flagged e2_flagged (Do_Overflow_Check :: checkflags)
-        | Divide   => E_Binary_Operation_X ast_num op e1_flagged e2_flagged (Do_Division_Check :: Do_Overflow_Check :: checkflags)
-        | _        => E_Binary_Operation_X ast_num op e1_flagged e2_flagged checkflags
+        | Plus     => E_Binary_Operation_X ast_num op e1_flagged e2_flagged (Do_Overflow_Check :: nil) nil
+        | Minus    => E_Binary_Operation_X ast_num op e1_flagged e2_flagged (Do_Overflow_Check :: nil) nil
+        | Multiply => E_Binary_Operation_X ast_num op e1_flagged e2_flagged (Do_Overflow_Check :: nil) nil
+        | Divide   => E_Binary_Operation_X ast_num op e1_flagged e2_flagged (Do_Division_Check :: Do_Overflow_Check :: nil) nil
+        | _        => E_Binary_Operation_X ast_num op e1_flagged e2_flagged nil nil
         end
   | E_Unary_Operation ast_num op e => 
-      let e_flagged := compile2_flagged_exp_f st nil e in
+      let e_flagged := compile2_flagged_exp_f st e in
         match op with
-        | Unary_Minus => E_Unary_Operation_X ast_num op e_flagged (Do_Overflow_Check :: checkflags)
-        | _           => E_Unary_Operation_X ast_num op e_flagged checkflags
+        | Unary_Minus => E_Unary_Operation_X ast_num op e_flagged (Do_Overflow_Check :: nil) nil
+        | _           => E_Unary_Operation_X ast_num op e_flagged nil nil
         end
   end
 
-with compile2_flagged_name_f (st: symboltable) (checkflags: check_flags) (n: name): name_x :=
+with compile2_flagged_name_f (st: symboltable) (n: name): name_x :=
   match n with
   | E_Identifier ast_num x =>
-        E_Identifier_X ast_num x checkflags
-  | E_Indexed_Component ast_num x_ast_num x e =>
-      let e_flagged := compile2_flagged_exp_f st (Do_Range_Check :: nil) e in
-        E_Indexed_Component_X ast_num x_ast_num x e_flagged checkflags
-  | E_Selected_Component ast_num x_ast_num x f =>
-        E_Selected_Component_X ast_num x_ast_num x f checkflags
+      E_Identifier_X ast_num x nil
+  | E_Indexed_Component ast_num x e =>
+      let x_flagged := compile2_flagged_name_f st x in
+      let e_flagged := compile2_flagged_exp_f st e in
+        E_Indexed_Component_X ast_num x_flagged (update_exterior_checks_exp e_flagged (Do_Range_Check :: nil)) nil
+  | E_Selected_Component ast_num x f =>
+      let x_flagged := compile2_flagged_name_f st x in
+        E_Selected_Component_X ast_num x_flagged f nil
   end.
-
 
 Function compile2_flagged_args_f (st: symboltable) (params: list parameter_specification) (args: list expression): option (list expression_x) :=
   match params, args with
   | nil, nil => Some nil
-  | param :: params', arg :: args' =>
-      match param.(parameter_mode) with
-      | In =>
-        if is_range_constrainted_type (param.(parameter_subtype_mark)) then
-          let arg_flagged := compile2_flagged_exp_f st (Do_Range_Check :: nil) arg in
-            match compile2_flagged_args_f st params' args' with
-            | Some args_flagged => Some (arg_flagged :: args_flagged)
-            | None              => None
-            end
-        else
-          let arg_flagged := compile2_flagged_exp_f st nil arg in
-            match compile2_flagged_args_f st params' args' with
-            | Some args_flagged => Some (arg_flagged :: args_flagged)
-            | None              => None
-            end 
-      | Out =>
-        match arg with
-        | E_Name ast_num (E_Identifier x_ast_num x) =>
-            match fetch_exp_type ast_num st with
-            | Some t =>
-                if is_range_constrainted_type t then
-                  let x_flagged := compile2_flagged_exp_f st (Do_Range_Check_On_CopyOut :: nil) (E_Name ast_num (E_Identifier x_ast_num x)) in
-                    match compile2_flagged_args_f st params' args' with
-                    | Some args_flagged => Some (x_flagged :: args_flagged)
-                    | None              => None
-                    end
-                else
-                  let x_flagged := compile2_flagged_exp_f st nil (E_Name ast_num (E_Identifier x_ast_num x)) in
-                    match compile2_flagged_args_f st params' args' with
-                    | Some args_flagged => Some (x_flagged :: args_flagged)
-                    | None              => None
-                    end
-            | None => None
-            end
-        | _ => None
-        end 
-      | In_Out => 
-        match arg with
-        | E_Name ast_num (E_Identifier x_ast_num x) =>
+  | param :: lparam, arg :: larg =>
+      match (compile2_flagged_args_f st lparam larg) with
+      | Some larg_flagged => 
+          match param.(parameter_mode) with
+          | In =>
+            let arg_flagged := compile2_flagged_exp_f st arg in
             if is_range_constrainted_type (param.(parameter_subtype_mark)) then
-              match fetch_exp_type ast_num st with
-              | Some t =>
-                  if is_range_constrainted_type t then
-                    let x_flagged := compile2_flagged_exp_f st (Do_Range_Check :: Do_Range_Check_On_CopyOut :: nil) 
-                                                               (E_Name ast_num (E_Identifier x_ast_num x)) in
-                      match compile2_flagged_args_f st params' args' with
-                      | Some args_flagged => Some (x_flagged :: args_flagged)
-                      | None              => None
-                      end
-                  else
-                    let x_flagged := compile2_flagged_exp_f st (Do_Range_Check :: nil) 
-                                                               (E_Name ast_num (E_Identifier x_ast_num x)) in
-                      match compile2_flagged_args_f st params' args' with
-                      | Some args_flagged => Some (x_flagged :: args_flagged)
-                      | None              => None
-                      end
-              | None => None
-              end
+              Some ((update_exterior_checks_exp arg_flagged (Do_Range_Check :: nil)) :: larg_flagged)
             else
-              match fetch_exp_type ast_num st with
-              | Some t =>
-                  if is_range_constrainted_type t then
-                    let x_flagged := compile2_flagged_exp_f st (Do_Range_Check_On_CopyOut :: nil) 
-                                                               (E_Name ast_num (E_Identifier x_ast_num x)) in
-                      match compile2_flagged_args_f st params' args' with
-                      | Some args_flagged => Some (x_flagged :: args_flagged)
-                      | None              => None
-                      end
-                  else
-                    let x_flagged := compile2_flagged_exp_f st nil 
-                                                               (E_Name ast_num (E_Identifier x_ast_num x)) in
-                      match compile2_flagged_args_f st params' args' with
-                      | Some args_flagged => Some (x_flagged :: args_flagged)
-                      | None              => None
-                      end
-              | None => None
-              end
-
-        | _ => None
-        end
+              Some (arg_flagged :: larg_flagged)
+          | Out =>
+            match arg with
+            | E_Name ast_num n =>
+                match fetch_exp_type ast_num st with
+                | Some t =>
+                    let n_flagged := compile2_flagged_name_f st n in
+                    if is_range_constrainted_type t then
+                      Some ((E_Name_X ast_num (update_exterior_checks_name n_flagged (Do_Range_Check_On_CopyOut :: nil))) :: larg_flagged)
+                    else
+                      Some ((E_Name_X ast_num n_flagged) :: larg_flagged)
+                | None => None
+                end
+            | _ => None
+            end
+          | In_Out =>
+            match arg with
+            | E_Name ast_num n =>
+                match fetch_exp_type ast_num st with
+                | Some t =>
+                    let n_flagged := compile2_flagged_name_f st n in
+                    if is_range_constrainted_type (param.(parameter_subtype_mark)) then 
+                      if is_range_constrainted_type t then
+                        Some ((E_Name_X ast_num (update_exterior_checks_name n_flagged (Do_Range_Check :: Do_Range_Check_On_CopyOut :: nil))) :: larg_flagged)
+                      else
+                        Some ((E_Name_X ast_num (update_exterior_checks_name n_flagged (Do_Range_Check :: nil))) :: larg_flagged)
+                    else
+                      if is_range_constrainted_type t then
+                        Some ((E_Name_X ast_num (update_exterior_checks_name n_flagged (Do_Range_Check_On_CopyOut :: nil))) :: larg_flagged)
+                      else
+                        Some ((E_Name_X ast_num n_flagged) :: larg_flagged)
+                | _ => None
+                end
+            | _ => None
+            end
+          end
+      | _ => None
       end
   | _, _ => None
   end.
@@ -462,33 +440,32 @@ Function compile2_flagged_stmt_f (st: symboltable) (c: statement): option statem
   match c with
   | S_Null => Some S_Null_X
   | S_Assignment ast_num x e =>
-      match fetch_exp_type (name_astnum x) st with
-      | Some t =>
+      let x_flagged := compile2_flagged_name_f st x in
+      let e_flagged := compile2_flagged_exp_f  st e in
+        match fetch_exp_type (name_astnum x) st with
+        | Some t =>
           if is_range_constrainted_type t then
-            let x_flagged := compile2_flagged_name_f st nil x in
-            let e_flagged := compile2_flagged_exp_f  st (Do_Range_Check :: nil) e in
-              Some (S_Assignment_X ast_num x_flagged e_flagged) 
+            Some (S_Assignment_X ast_num x_flagged (update_exterior_checks_exp e_flagged (Do_Range_Check :: nil)))
           else
-            let x_flagged := compile2_flagged_name_f st nil x in
-            let e_flagged := compile2_flagged_exp_f  st nil e in
-              Some (S_Assignment_X ast_num x_flagged e_flagged)
-      | None   => None
-      end
+            Some (S_Assignment_X ast_num x_flagged e_flagged)
+        | None   => None
+        end
   | S_If ast_num e c1 c2 =>
-      let e_flagged := compile2_flagged_exp_f st nil e in
-        match compile2_flagged_stmt_f st c1 with
-        | Some c1_flagged =>
-            match compile2_flagged_stmt_f st c2 with
-            | Some c2_flagged => Some (S_If_X ast_num e_flagged c1_flagged c2_flagged)
-            | None            => None
-            end
-        | None            => None
+      let e_flagged  := compile2_flagged_exp_f st e in
+      let c1' := compile2_flagged_stmt_f st c1 in
+      let c2' := compile2_flagged_stmt_f st c2 in
+        match (c1', c2') with 
+        | (Some c1_flagged, Some c2_flagged) => 
+            Some (S_If_X ast_num e_flagged c1_flagged c2_flagged)
+        | _ => None
         end
   | S_While_Loop ast_num e c =>
-      let e_flagged := compile2_flagged_exp_f st nil e in
-        match compile2_flagged_stmt_f st c with
-        | Some c_flagged => Some (S_While_Loop_X ast_num e_flagged c_flagged)
-        | None           => None
+      let e_flagged := compile2_flagged_exp_f st e in
+      let c' := compile2_flagged_stmt_f st c in
+        match c' with 
+        | Some c_flagged => 
+            Some (S_While_Loop_X ast_num e_flagged c_flagged)
+        | _ => None
         end
   | S_Procedure_Call ast_num p_ast_num p args =>
       match fetch_proc p st with
@@ -500,13 +477,12 @@ Function compile2_flagged_stmt_f (st: symboltable) (c: statement): option statem
       | None         => None
       end
   | S_Sequence ast_num c1 c2 =>
-      match compile2_flagged_stmt_f st c1 with
-      | Some c1_flagged =>
-          match compile2_flagged_stmt_f st c2 with
-          | Some c2_flagged => Some (S_Sequence_X ast_num c1_flagged c2_flagged)
-          | None            => None
-          end
-      | None            => None
+      let c1' := compile2_flagged_stmt_f st c1 in
+      let c2' := compile2_flagged_stmt_f st c2 in
+      match (c1', c2') with
+      | (Some c1_flagged, Some c2_flagged) =>
+          Some (S_Sequence_X ast_num c1_flagged c2_flagged)
+      | _ => None
       end
   end.
 
@@ -518,22 +494,21 @@ Function compile2_flagged_type_declaration_f (t: type_declaration): type_declara
       Derived_Type_Declaration_X ast_num tn t (Range_X l u)
   | Integer_Type_Declaration ast_num tn (Range l u) =>
       Integer_Type_Declaration_X ast_num tn (Range_X l u)
-  | Array_Type_Declaration ast_num tn tm t => 
+  | Array_Type_Declaration ast_num tn tm t => (* tn: array type name, tm: index type mark, t: component type *)
       Array_Type_Declaration_X ast_num tn tm t
-  | Record_Type_Declaration ast_num tn fs =>
+  | Record_Type_Declaration ast_num tn fs =>  (* tn: record type name, fs: list of field types *)
       Record_Type_Declaration_X ast_num tn fs
   end.
 
 Function compile2_flagged_object_declaration_f (st: symboltable) (o: object_declaration): object_declaration_x :=
   match o with
   | mkobject_declaration ast_num x t None =>
-        mkobject_declaration_x ast_num x t None
+      mkobject_declaration_x ast_num x t None
   | mkobject_declaration ast_num x t (Some e) => 
-      if is_range_constrainted_type t then
-        let e_flagged := compile2_flagged_exp_f st (Do_Range_Check :: nil) e in
-          mkobject_declaration_x ast_num x t (Some e_flagged) 
-      else
-        let e_flagged := compile2_flagged_exp_f st nil e in
+      let e_flagged := compile2_flagged_exp_f st e in
+        if is_range_constrainted_type t then
+          mkobject_declaration_x ast_num x t (Some (update_exterior_checks_exp e_flagged (Do_Range_Check :: nil)))
+        else
           mkobject_declaration_x ast_num x t (Some e_flagged)
   end.
 
@@ -569,7 +544,7 @@ Function compile2_flagged_declaration_f (st: symboltable) (d: declaration): opti
       let t_flagged := compile2_flagged_type_declaration_f t in
         Some (D_Type_Declaration_X ast_num t_flagged)
   | D_Object_Declaration ast_num o =>
-      let o_flagged := compile2_flagged_object_declaration_f st o in
+      let o_flagged := compile2_flagged_object_declaration_f st o in 
         Some (D_Object_Declaration_X ast_num o_flagged)
   | D_Procedure_Body ast_num p =>
       match compile2_flagged_procedure_body_f st p with
@@ -577,13 +552,11 @@ Function compile2_flagged_declaration_f (st: symboltable) (d: declaration): opti
       | None           => None
       end
   | D_Seq_Declaration ast_num d1 d2 =>
-      match compile2_flagged_declaration_f st d1 with
-      | Some d1_flagged =>
-          match compile2_flagged_declaration_f st d2 with
-          | Some d2_flagged => Some (D_Seq_Declaration_X ast_num d1_flagged d2_flagged)
-          | None            => None
-          end
-      | None                => None
+      let d1' := compile2_flagged_declaration_f st d1 in
+      let d2' := compile2_flagged_declaration_f st d2 in
+      match (d1', d2') with 
+      | (Some d1_flagged, Some d2_flagged) => Some (D_Seq_Declaration_X ast_num d1_flagged d2_flagged)
+      | _ => None
       end
   end
 
@@ -591,14 +564,12 @@ with compile2_flagged_procedure_body_f (st: symboltable) (p: procedure_body): op
   match p with
   | mkprocedure_body ast_num p params decls stmt =>
       let params_flagged := compile2_flagged_parameter_specifications_f params in
-        match compile2_flagged_declaration_f st decls with
-        | Some decls_flagged =>
-          match compile2_flagged_stmt_f st stmt with
-          | Some stmt_flagged => Some (mkprocedure_body_x ast_num p params_flagged decls_flagged stmt_flagged)
-          | None              => None
-          end
-        | None                => None
-        end
+      let decls' := compile2_flagged_declaration_f st decls in
+      let stmt' := compile2_flagged_stmt_f st stmt in
+      match (decls', stmt') with 
+      | (Some decls_flagged, Some stmt_flagged) => Some (mkprocedure_body_x ast_num p params_flagged decls_flagged stmt_flagged)
+      | _ => None
+      end
   end.
 
 
@@ -613,32 +584,40 @@ Scheme expression_ind := Induction for expression Sort Prop
 
 Section Checks_Generator_Function_Correctness_Proof.
 
-  Lemma compile2_flagged_exp_f_correctness: forall e e' checkflags st,
-    compile2_flagged_exp_f st checkflags e = e' ->
-      compile2_flagged_exp st checkflags e e'.
+  Lemma compile2_flagged_exp_f_correctness: forall e e' st,
+    compile2_flagged_exp_f st e = e' ->
+      compile2_flagged_exp st e e'.
   Proof.
     apply (expression_ind
-      (fun e: expression => forall (e' : expression_x) (checkflags: check_flags) (st: symboltable),
-        compile2_flagged_exp_f st checkflags e = e' ->
-        compile2_flagged_exp   st checkflags e e')
-      (fun n: name => forall (n': name_x) (checkflags: check_flags) (st: symboltable),
-        compile2_flagged_name_f st checkflags n = n' ->
-        compile2_flagged_name   st checkflags n n')
+      (fun e: expression => forall (e' : expression_x) (st: symboltable),
+        compile2_flagged_exp_f st e = e' ->
+        compile2_flagged_exp   st e e')
+      (fun n: name => forall (n': name_x) (st: symboltable),
+        compile2_flagged_name_f st n = n' ->
+        compile2_flagged_name   st n n')
       ); smack;
-    [ | | 
-      destruct b; constructor; smack | 
-      destruct u; constructor; smack | | | 
-    ];
-    constructor; apply H; auto.
+    [ (*E_Literal*) 
+      destruct l;
+      [ remember ((z >=? min_signed)%Z && (z <=? max_signed)%Z) as b; destruct b;
+        smack; constructor; smack |
+        smack; constructor
+      ] | 
+      (*E_Name*) | 
+      (*E_Binary_Operation a b e e0*) destruct b |
+      (*E_Unary_Operation a u e*) destruct u |
+      (*E_Identifier a i*) |
+      (*E_Indexed_Component a n e*) |
+      (*E_Selected_Component a n i*)
+    ]; 
+    constructor; smack.
   Qed.
 
-  Lemma compile2_flagged_name_f_correctness: forall st checkflags n n',
-    compile2_flagged_name_f st checkflags n = n' ->
-      compile2_flagged_name st checkflags n n'.
+  Lemma compile2_flagged_name_f_correctness: forall st n n',
+    compile2_flagged_name_f st n = n' ->
+      compile2_flagged_name st n n'.
   Proof.
-    intros.
-    destruct n; smack;
-    repeat progress constructor;
+    intros st n;
+    induction n; smack; constructor; smack;
     apply compile2_flagged_exp_f_correctness; auto.
   Qed.
 
@@ -647,39 +626,41 @@ Section Checks_Generator_Function_Correctness_Proof.
       compile2_flagged_args st params args args'.
   Proof.
     induction params; smack.
-  - destruct args; smack.
+  - destruct args; smack;
     constructor.
   - destruct args; smack.
-    remember (parameter_mode a) as m; destruct m.
-    + remember (is_range_constrainted_type (parameter_subtype_mark a)) as x;
-      remember (compile2_flagged_args_f st params args) as y;
-      destruct x, y; smack;
-      [apply C2_Flagged_Args_In_Range; smack |
-       apply C2_Flagged_Args_In; smack
-      ]; apply compile2_flagged_exp_f_correctness; auto.
-    + destruct e; smack.
-      destruct n; smack.
-      remember (fetch_exp_type a0 st) as x;
-      destruct x; smack.
-      remember (is_range_constrainted_type t) as y;
-      remember (compile2_flagged_args_f st params args) as z;
-      destruct y, z; smack;
-      [apply C2_Flagged_Args_Out_Range with (t := t); auto |
-       apply C2_Flagged_Args_Out with (t := t); auto
-      ]; apply compile2_flagged_exp_f_correctness; auto.
-    + destruct e; smack.
-      destruct n; smack.
+    remember (compile2_flagged_args_f st params args) as b1;
+    remember (parameter_mode a) as b2; 
+    destruct b1, b2; smack.
+    + (*In Mode*)
       remember (is_range_constrainted_type (parameter_subtype_mark a)) as x;
-      remember (fetch_exp_type a0 st) as y;
-      destruct x, y; smack;
-      remember (is_range_constrainted_type t) as z;
-      remember (compile2_flagged_args_f st params args) as w;
-      destruct z, w; smack;
-      [ apply C2_Flagged_Args_InOut_Range with (t := t); auto     |
-        apply C2_Flagged_Args_InOut_In_Range with (t := t); auto  |
-        apply C2_Flagged_Args_InOut_Out_Range with (t := t); auto |
-        apply C2_Flagged_Args_InOut with (t := t); auto
-      ]; apply compile2_flagged_exp_f_correctness; auto.
+      destruct x; smack;
+      [ apply C2_Flagged_Args_In_RangeCheck |
+        apply C2_Flagged_Args_In
+      ]; smack; 
+      apply compile2_flagged_exp_f_correctness; auto.
+    + (*Out Mode*)
+      destruct e; smack;
+      remember (fetch_exp_type a0 st) as b3;
+      destruct b3; smack;
+      remember (is_range_constrainted_type t) as b4; destruct b4; smack;
+      [ apply C2_Flagged_Args_Out_RangeCheck with (t := t) |
+        apply C2_Flagged_Args_Out with (t := t)
+      ]; smack;
+      apply compile2_flagged_name_f_correctness; auto.
+    + (*In_Out Mode*)
+      destruct e; smack;
+      remember (is_range_constrainted_type (parameter_subtype_mark a)) as b3;
+      remember (fetch_exp_type a0 st) as b4;
+      destruct b3, b4; smack;
+      remember (is_range_constrainted_type t) as b5;
+      destruct b5; smack;
+      [ apply C2_Flagged_Args_InOut_RangeCheck with (t:=t) |
+        apply C2_Flagged_Args_InOut_In_RangeCheck with (t:=t) |
+        apply C2_Flagged_Args_InOut_Out_RangeCheck with (t:=t) |
+        apply C2_Flagged_Args_InOut with (t:=t)
+      ]; auto;
+      apply compile2_flagged_name_f_correctness; auto.
   Qed.
 
   Lemma compile2_flagged_stmt_f_correctness: forall st c c',
@@ -687,41 +668,43 @@ Section Checks_Generator_Function_Correctness_Proof.
       compile2_flagged_stmt st c c'.
   Proof.
     induction c; smack.
-  - constructor.
-  - remember (fetch_exp_type (name_astnum n) st) as x;
-    destruct x; smack.
-    remember (is_range_constrainted_type t) as y.
-    destruct y; smack;
-    [apply C2_Flagged_Assignment_R with (t := t); smack |
-     apply C2_Flagged_Assignment with (t := t); smack 
-    ];
-    [apply compile2_flagged_name_f_correctness; auto | | 
-     apply compile2_flagged_name_f_correctness; auto | 
-    ];
+  - (*S_Null*)
+    constructor.
+  - (*S_Assignment*)
+    remember (fetch_exp_type (name_astnum n) st ) as b1;
+    destruct b1; smack;
+    remember (is_range_constrainted_type t) as b2;
+    destruct b2; smack;
+    [ apply C2_Flagged_Assignment_RangeCheck with (t := t) |
+      apply C2_Flagged_Assignment with (t := t)
+    ]; auto;
+    solve 
+    [ apply compile2_flagged_name_f_correctness; auto |
+      apply compile2_flagged_exp_f_correctness; auto
+    ].
+  - (*S_If*)
+    remember (compile2_flagged_stmt_f st c1) as b1;
+    remember (compile2_flagged_stmt_f st c2) as b2;
+    destruct b1, b2; smack;
+    constructor; smack;
     apply compile2_flagged_exp_f_correctness; auto.
-  - remember (compile2_flagged_stmt_f st c1) as x;
-    destruct x; smack.
-    remember (compile2_flagged_stmt_f st c2) as y;
-    destruct y; smack.
-    constructor;
-    [ apply compile2_flagged_exp_f_correctness | | ];
-    smack.
-  - remember (compile2_flagged_stmt_f st c) as x;
-    destruct x; smack.
-    constructor;
-    [ apply compile2_flagged_exp_f_correctness | ];
-    smack.
-  - remember (fetch_proc p st) as x;
-    destruct x; smack.
-    destruct t.
-    remember (compile2_flagged_args_f st (procedure_parameter_profile p0) l) as y;
-    destruct y; smack.
-    apply C2_Flagged_Procedure_Call with (n := l0) (pb := p0) (params := (procedure_parameter_profile p0)); smack.
+  - (*S_While_Loop*)
+    remember (compile2_flagged_stmt_f st c) as b1;
+    destruct b1; smack;
+    constructor; smack;
+    apply compile2_flagged_exp_f_correctness; auto.
+  - (*S_Procedure_Call*)
+    remember (fetch_proc p st) as b1;
+    destruct b1; smack;
+    destruct t;
+    remember (compile2_flagged_args_f st (procedure_parameter_profile p0) l) as b2;
+    destruct b2; smack;
+    apply C2_Flagged_Procedure_Call with (n := l0) (pb := p0) (params := (procedure_parameter_profile p0)); smack;
     apply compile2_flagged_args_f_correctness; auto.
-  - remember (compile2_flagged_stmt_f st c1) as x;
-    destruct x; smack.
-    remember (compile2_flagged_stmt_f st c2) as y;
-    destruct y; smack.
+  - (*S_Sequence*)
+    remember (compile2_flagged_stmt_f st c1) as b1;
+    remember (compile2_flagged_stmt_f st c2) as b2;
+    destruct b1, b2; smack;
     constructor; auto.
   Qed.
 
@@ -739,20 +722,19 @@ Section Checks_Generator_Function_Correctness_Proof.
   Proof.
     intros;
     functional induction compile2_flagged_object_declaration_f st o; smack;
-    [constructor |
-     apply C2_Flagged_Object_Declaration_R; auto |
-     apply C2_Flagged_Object_Declaration; auto
-    ];
-    apply compile2_flagged_exp_f_correctness; auto.
+    [ constructor |
+      apply C2_Flagged_Object_Declaration_RangeCheck |
+      apply C2_Flagged_Object_Declaration 
+    ]; auto; apply compile2_flagged_exp_f_correctness; auto.
   Qed.
 
   Lemma compile2_flagged_object_declarations_f_correctness: forall st lo lo',
     compile2_flagged_object_declarations_f st lo = lo' ->
       compile2_flagged_object_declarations st lo lo'.
   Proof.
-    induction lo; smack; 
-    constructor; smack.
-    apply compile2_flagged_object_declaration_f_correctness; auto.   
+    induction lo; smack;
+    constructor; smack;
+    apply compile2_flagged_object_declaration_f_correctness; auto.
   Qed.
 
   Lemma compile2_flagged_parameter_specification_f_correctness: forall param param',
@@ -769,7 +751,7 @@ Section Checks_Generator_Function_Correctness_Proof.
       compile2_flagged_parameter_specifications lparam lparam'.
   Proof.
     induction lparam; smack;
-    constructor; smack.
+    constructor; smack;
     apply compile2_flagged_parameter_specification_f_correctness; auto.
   Qed.
 
@@ -790,20 +772,20 @@ Section Checks_Generator_Function_Correctness_Proof.
         compile2_flagged_procedure_body st p p')
       ); smack.
   - constructor.
-  - constructor.
+  - constructor;
     apply compile2_flagged_type_declaration_f_correctness; auto.
-  - constructor.
+  - constructor;
     apply compile2_flagged_object_declaration_f_correctness; auto.
   - remember (compile2_flagged_procedure_body_f st p) as x; 
-    destruct x; smack.
+    destruct x; smack;
     constructor; auto.
   - remember (compile2_flagged_declaration_f st d) as x;
     remember (compile2_flagged_declaration_f st d0) as y;
-    destruct x, y; smack.  
+    destruct x, y; smack;
     constructor; smack.
   - remember (compile2_flagged_declaration_f st procedure_declarative_part) as x;
     remember (compile2_flagged_stmt_f st procedure_statements) as y;
-    destruct x, y; smack.
+    destruct x, y; smack;
     constructor;
     [ apply compile2_flagged_parameter_specifications_f_correctness | |
       apply compile2_flagged_stmt_f_correctness
@@ -818,7 +800,7 @@ Section Checks_Generator_Function_Correctness_Proof.
     destruct p; smack.
     remember (compile2_flagged_declaration_f st procedure_declarative_part) as x;
     remember (compile2_flagged_stmt_f st procedure_statements) as y;
-    destruct x, y; smack.  
+    destruct x, y; smack;
     constructor;
     [ apply compile2_flagged_parameter_specifications_f_correctness |
       apply compile2_flagged_declaration_f_correctness |
@@ -831,47 +813,47 @@ End Checks_Generator_Function_Correctness_Proof.
 
 Section Checks_Generator_Function_Completeness_Proof.
 
-  Lemma compile2_flagged_exp_f_completeness: forall e e' checkflags st,
-    compile2_flagged_exp st checkflags e e' ->
-      compile2_flagged_exp_f st checkflags e = e'.
+  Lemma compile2_flagged_exp_f_completeness: forall e e' st,
+    compile2_flagged_exp st e e' ->
+      compile2_flagged_exp_f st e = e'.
   Proof.
     apply (expression_ind
-      (fun e: expression => forall (e' : expression_x) (checkflags: check_flags) (st: symboltable),
-        compile2_flagged_exp   st checkflags e e' ->
-        compile2_flagged_exp_f st checkflags e = e')
-      (fun n: name => forall (n': name_x) (checkflags: check_flags) (st: symboltable),
-        compile2_flagged_name   st checkflags n n' ->
-        compile2_flagged_name_f st checkflags n = n')
+      (fun e: expression => forall (e' : expression_x) (st: symboltable),
+        compile2_flagged_exp   st e e' ->
+        compile2_flagged_exp_f st e = e')
+      (fun n: name => forall (n': name_x) (st: symboltable),
+        compile2_flagged_name   st n n' ->
+        compile2_flagged_name_f st n = n')
       ); smack;
     match goal with
-    | [H: compile2_flagged_exp  _ _ ?e ?e' |- _] => inversion H; clear H; smack
-    | [H: compile2_flagged_name _ _ ?n ?n' |- _] => inversion H; clear H; smack
+    | [H: compile2_flagged_exp  _ ?e ?e' |- _] => inversion H; clear H; smack
+    | [H: compile2_flagged_name _ ?n ?n' |- _] => inversion H; clear H; smack
     end;
     repeat progress match goal with
-    | [H1:forall (e' : expression_x) (checkflags : check_flags) (st : symboltable),
-          compile2_flagged_exp _ _ ?e e' ->
-          compile2_flagged_exp_f _ _ ?e = e',
-       H2:compile2_flagged_exp _ _ ?e ?e1_flagged |- _] => specialize (H1 _ _ _ H2); smack
-    | [H1:forall (n' : name_x) (checkflags : check_flags) (st : symboltable),
-          compile2_flagged_name _ _ ?n n' ->
-          compile2_flagged_name_f _ _ ?n = n',
-       H2:compile2_flagged_name _ _ ?n ?n_flagged |- _] => specialize (H1 _ _ _ H2); smack
-    end; 
-    [ destruct b |
-      destruct u
+    | [H1:forall (e' : expression_x) (st : symboltable),
+          compile2_flagged_exp _ ?e e' ->
+          compile2_flagged_exp_f _ ?e = e',
+       H2:compile2_flagged_exp _ ?e ?e1_flagged |- _] => specialize (H1 _ _ H2); smack
+    | [H1:forall (n' : name_x) (st : symboltable),
+          compile2_flagged_name _ ?n n' ->
+          compile2_flagged_name_f _ ?n = n',
+       H2:compile2_flagged_name _ ?n ?n_flagged |- _] => specialize (H1 _ _ H2); smack
+    end;
+    [ destruct b | 
+      destruct u 
     ]; smack.
   Qed.
 
-  Lemma compile2_flagged_name_f_completeness: forall st checkflags n n',
-    compile2_flagged_name st checkflags n n' ->
-      compile2_flagged_name_f st checkflags n = n'.
+  Lemma compile2_flagged_name_f_completeness: forall st n n',
+    compile2_flagged_name st n n' ->
+      compile2_flagged_name_f st n = n'.
   Proof.
-    intros.
-    destruct n;
+    intros;
+    induction H; smack;
     match goal with
-    | [H: compile2_flagged_name _ _ ?n ?n' |- _] => inversion H; clear H; smack
-    end.
-    specialize (compile2_flagged_exp_f_completeness _ _ _ _ H7); smack.
+    | [H: compile2_flagged_exp ?st ?e ?e' |- _] => 
+        specialize (compile2_flagged_exp_f_completeness _ _ _ H); smack
+    end; auto.
   Qed.
 
   Lemma compile2_flagged_args_f_completeness: forall st params args args',
@@ -889,8 +871,13 @@ Section Checks_Generator_Function_Completeness_Proof.
        H2: compile2_flagged_args _ ?params _ _ |- _] => specialize (H1 _ _ H2)
     end;
     match goal with
-    | [H: compile2_flagged_exp _ _ ?e ?e' |- _] => specialize (compile2_flagged_exp_f_completeness _ _ _ _ H); smack
-    end.
+    | [H: compile2_flagged_args_f ?st ?params ?larg = Some _ |- _] => rewrite H; simpl
+    end;
+    match goal with
+    | [H: compile2_flagged_exp _ ?e ?e' |- _] => specialize (compile2_flagged_exp_f_completeness _ _ _ H); smack
+    | [H: compile2_flagged_name _ ?n ?n' |- _] => specialize (compile2_flagged_name_f_completeness _ _ _ H); smack
+    | _ => idtac
+    end; auto.
   Qed.
 
   Lemma compile2_flagged_stmt_f_completeness: forall st c c',
@@ -902,16 +889,16 @@ Section Checks_Generator_Function_Completeness_Proof.
     | [H: compile2_flagged_stmt _ ?c ?c' |- _] => inversion H; clear H; smack
     end;
     repeat progress match goal with
-    | [H: compile2_flagged_exp  _ _ ?e ?e' |- _] => specialize (compile2_flagged_exp_f_completeness  _ _ _ _ H); clear H
-    | [H: compile2_flagged_name _ _ ?n ?n' |- _] => specialize (compile2_flagged_name_f_completeness _ _ _ _ H); clear H
+    | [H: compile2_flagged_exp  _ ?e ?e' |- _] => specialize (compile2_flagged_exp_f_completeness  _ _ _ H); clear H
+    | [H: compile2_flagged_name _ ?n ?n' |- _] => specialize (compile2_flagged_name_f_completeness _ _ _ H); clear H
     | [H1: forall c' : statement_x,
            compile2_flagged_stmt _ ?c _ ->
            compile2_flagged_stmt_f _ ?c = Some _,
        H2: compile2_flagged_stmt _ ?c _ |- _ ] => specialize (H1 _ H2)
-    end; smack.
-     match goal with
-    | [H: compile2_flagged_args _ _ _ _ |- _ ] => specialize (compile2_flagged_args_f_completeness _ _ _ _ H)
-    end; smack.
+    end; smack;
+    match goal with
+    | [H: compile2_flagged_args _ _ _ _ |- _ ] => specialize (compile2_flagged_args_f_completeness _ _ _ _ H); smack
+    end.
   Qed.
 
   Lemma compile2_flagged_type_declaration_f_completeness: forall t t',
@@ -934,9 +921,9 @@ Section Checks_Generator_Function_Completeness_Proof.
     | [H: compile2_flagged_object_declaration _ _ _ |- _] => inversion H; smack
     end;
     match goal with
-    | [H: compile2_flagged_exp _ _ _ _ |- _] => 
-        specialize (compile2_flagged_exp_f_completeness _ _ _ _ H); smack
-    end.
+    | [H: compile2_flagged_exp _ _ _ |- _] => 
+        specialize (compile2_flagged_exp_f_completeness _ _ _ H); smack
+    end. 
   Qed.
 
   Lemma compile2_flagged_object_declarations_f_completeness: forall st lo lo',
@@ -967,8 +954,8 @@ Section Checks_Generator_Function_Completeness_Proof.
       compile2_flagged_parameter_specifications_f lparam = lparam'.
   Proof.
     induction lparam; intros;
-    inversion H; auto.
-    specialize (IHlparam _ H4).
+    inversion H; auto;
+    specialize (IHlparam _ H4);
     match goal with
     | [H: compile2_flagged_parameter_specification _ _ |- _] => 
         specialize (compile2_flagged_parameter_specification_f_completeness _ _ H); smack
@@ -1018,7 +1005,7 @@ Section Checks_Generator_Function_Completeness_Proof.
       compile2_flagged_procedure_body_f st p = Some p'.
   Proof.
     intros;
-    destruct p.
+    destruct p;
     match goal with
     [H: compile2_flagged_procedure_body _ _ _ |- _] => inversion H; clear H; smack
     end;
@@ -1038,6 +1025,42 @@ End Checks_Generator_Function_Completeness_Proof.
 (** * Lemmas *)
 
 Require Import CpdtTactics.
+
+Lemma exp_ast_num_eq: forall st e e',
+  compile2_flagged_exp st e e' ->
+    expression_astnum e = expression_astnum_x e'.
+Proof.
+  intros; inversion H; smack.
+Qed.
+
+Lemma name_ast_num_eq: forall st n n',
+  compile2_flagged_name st n n' ->
+    name_astnum n = name_astnum_x n'.
+Proof.
+  intros; inversion H; smack.
+Qed.
+
+Lemma exp_exterior_checks_beq_nil: forall st e e',
+  compile2_flagged_exp st e e' ->
+    exp_exterior_checks e' = nil.
+Proof.
+  intros; 
+  inversion H; smack;
+  inversion H; subst;
+  destruct n; 
+  match goal with
+  | [H: compile2_flagged_name _ _ _ |- _] => inversion H; smack
+  end.
+Qed.
+
+Lemma name_exterior_checks_beq_nil: forall st n n',
+  compile2_flagged_name st n n' ->
+    name_exterior_checks n' = nil.
+Proof.
+  intros; 
+  inversion H; smack.
+Qed.
+
 
 Lemma procedure_components_rel: forall st p p',
   compile2_flagged_procedure_body st p p' ->
@@ -1073,10 +1096,10 @@ Inductive compile2_flagged_type_declaration_map: list (idnum * type_declaration)
         compile2_flagged_type_declaration_map ((x, t) :: tl) ((x, t') :: tl').
 
 Inductive compile2_flagged_symbol_table: symboltable -> symboltable_x -> Prop := 
-  | C2_Flagged_SymTable: forall p p' t t' x e srcloc,
-      compile2_flagged_proc_declaration_map (mkSymbolTable x p t e srcloc) p p' ->
+  | C2_Flagged_SymTable: forall p p' t t' x e srcloc nametable,
+      compile2_flagged_proc_declaration_map (mkSymbolTable x p t e srcloc nametable) p p' ->
       compile2_flagged_type_declaration_map t t' ->
-      compile2_flagged_symbol_table (mkSymbolTable x p t e srcloc) (mkSymbolTable_x x p' t' e srcloc).
+      compile2_flagged_symbol_table (mkSymbolTable x p t e srcloc nametable) (mkSymbolTable_x x p' t' e srcloc nametable).
 
 
 (** ** Lemmas *)
