spark2014_semantics/spark2014_core_subset/symboltable_module.v
@@ -1,6 +1,15 @@
 Require Export environment.
+Require Export Coq.Strings.String.
 
 (** * Symbol Table Elements *)
+
+Record nametable := mkNameTable{
+  varNames:  list (idnum * (string * string));
+  procNames: list (procnum * (string * string));
+  pkgNames: list (pkgnum * (string * string));
+  typeNames: list (typenum * (string * string))
+}.
+
 
 Module Type SymTable_Element.
 
@@ -32,6 +41,8 @@ Module SymbolTableM (S: SymTable_Element).
       - types: map each type name to its type declaration;
       - exps : record the type for each expression ast node;
       - sloc : map each ast node back to the source location in SPARK source code;
+      - names: map name id, represented as natural number, to a pair of (name string, unique name string),
+               e.g. 1 -> ("x", "ada://variable/pacakge_name/procedure_name_where_X_is_decalred/X+12:24")
   *)
  
   Record symboltable := mkSymbolTable{
@@ -39,10 +50,16 @@ Module SymbolTableM (S: SymTable_Element).
     procs: list (procnum * (level * proc_decl));
     types: list (typenum * type_decl);
     exps: list (astnum * type);
-    sloc: list (astnum * source_location)
-    (*used to map back to the source location once an error is detected in ast tree*)
+    sloc: list (astnum * source_location); (*used to map back to the source location once an error is detected in ast tree*)
+    names: nametable
   }.
 
+  (** name table entry *)
+  Module Entry_Name <: ENTRY.
+    Definition T := prod string string.
+  End Entry_Name.
+
+  (** symbol table entry *)
   Module Entry_Type <: ENTRY.
     Definition T := prod mode type.
   End Entry_Type.
@@ -63,12 +80,27 @@ Module SymbolTableM (S: SymTable_Element).
     Definition T := source_location.
   End Entry_Sloc.
 
-
+  (** name table module *)
+  Module Names  := STORE(Entry_Name).
+  
+  (** symbol table module *)
   Module SymTable_Vars  := STORE(Entry_Type).
   Module SymTable_Procs := STORE(Entry_Procedure_Decl).
   Module SymTable_Types := STORE(Entry_Type_Decl).
   Module SymTable_Exps := STORE(Entry_Exp_Type).
   Module SymTable_Sloc := STORE(Entry_Sloc).
+
+  (** ** Name Table Operations *)
+  Function reside_nametable_vars  (x: idnum)   (nt: nametable) := Names.resides x nt.(varNames).
+  Function reside_nametable_procs (x: procnum) (nt: nametable) := Names.resides x nt.(procNames).
+  Function reside_nametable_pkgs  (x: pkgnum)  (nt: nametable) := Names.resides x nt.(pkgNames).
+  Function reside_nametable_types (x: typenum) (nt: nametable) := Names.resides x nt.(typeNames).
+
+  Function fetch_var_name  (x: idnum)   (nt: nametable) := Names.fetches x nt.(varNames).
+  Function fetch_proc_name (x: procnum) (nt: nametable) := Names.fetches x nt.(procNames).
+  Function fetch_pkg_name  (x: pkgnum)  (nt: nametable) := Names.fetches x nt.(pkgNames).
+  Function fetch_type_name (x: typenum) (nt: nametable) := Names.fetches x nt.(typeNames).
+
 
   (** ** Symbol Table Operations *)
 
@@ -97,19 +129,22 @@ Module SymbolTableM (S: SymTable_Element).
   Arguments update_store {V} _ _ _.
 
   Function update_vars (st: symboltable) (x: idnum) (mt: mode * type): symboltable :=
-    mkSymbolTable (update_store st.(vars) x mt) st.(procs) st.(types) st.(exps) st.(sloc).
+    mkSymbolTable (update_store st.(vars) x mt) st.(procs) st.(types) st.(exps) st.(sloc) st.(names).
 
   Function update_procs (st: symboltable) (pid: procnum) (p: level * proc_decl): symboltable :=
-    mkSymbolTable st.(vars) (update_store st.(procs) pid p) st.(types) st.(exps) st.(sloc).
+    mkSymbolTable st.(vars) (update_store st.(procs) pid p) st.(types) st.(exps) st.(sloc) st.(names).
 
   Function update_types (st: symboltable) (tid: typenum) (td: type_decl): symboltable :=
-    mkSymbolTable st.(vars) st.(procs) (update_store st.(types) tid td) st.(exps) st.(sloc).
+    mkSymbolTable st.(vars) st.(procs) (update_store st.(types) tid td) st.(exps) st.(sloc) st.(names).
 
   Function update_exps (st: symboltable) (ast_num: astnum) (t: type): symboltable :=
-    mkSymbolTable st.(vars) st.(procs) st.(types) (update_store st.(exps) ast_num t) st.(sloc).
+    mkSymbolTable st.(vars) st.(procs) st.(types) (update_store st.(exps) ast_num t) st.(sloc) st.(names).
 
   Function update_sloc (st: symboltable) (ast_num: astnum) (sl: source_location): symboltable :=
-    mkSymbolTable st.(vars) st.(procs) st.(types) st.(exps) (update_store st.(sloc) ast_num sl).
+    mkSymbolTable st.(vars) st.(procs) st.(types) st.(exps) (update_store st.(sloc) ast_num sl) st.(names).
+
+  Function update_names (st: symboltable) (names: nametable): symboltable :=
+    mkSymbolTable st.(vars) st.(procs) st.(types) st.(exps) st.(sloc) names.
 
 End SymbolTableM.
 
